Clap/eDSLState/Varstore.lean
@@ -1,0 +1,8 @@
+import Mathlib.Data.ZMod.Basic
+import Std.Data.ExtTreeMap
+
+namespace Clap
+
+abbrev VarStore (p : ℕ) := Std.ExtTreeMap ℕ (ZMod p) (cmp := compare)
+
+end Clap
